4$$m_l(x) = \rho(x)I(x){\partial^2\Psi\over\partial t^2}$$
5$$\rho(x)={m(x)r(x)^2\over I(x)}$$
6$${\partial\over\partial x}\left(EI(x){\partial\Psi\over\partial x}\right) = k(x)GA(x)\left(\Psi - {\partial y\over\partial x}\right) + m(x)r(x)^2{\partial^2\Psi\over\partial t^2}$$
7$$kGA{\partial\over\partial x}\left(\Psi - {\partial y\over\partial x}\right) + m{\partial^2y\over\partial t^2} = 0$$
8$$EI{\partial\over\partial x}\left({\partial\Psi\over\partial x}\right) = kGA\left(\Psi - {\partial y\over\partial x}\right) + mr^2{\partial^2\Psi\over\partial t^2}$$
9$$EI{\partial^4 y\over\partial x^4} + m{\partial^2y\over\partial t^2} - {mEI\over kGA}{\partial^2\over\partial x^2}\left({\partial^2y\over\partial t^2}\right) - mr^2{\partial^2\over\partial x^2}\left({\partial^2y\over\partial t^2}\right) + {m^2r^2\over kGA}{\partial^4y\over\partial t^4} = 0$$
10$$y_{(x,t)} = \varphi(x)e^{i\omega t}$$
11$$EI\varphi^{(4)}(x)+\omega^2\left(mr^2+{mEI\over A_sG}\right)\varphi^{(2)}(x) + \left({m^2\omega^4r^2\over A_sG} - m\omega^2\right)\varphi(x) = 0$$
12$$a^2 = {EI\over A_sGL^2}$$
13$$b_n^2={m\omega^2L^4\over EI}$$
14$$R^2=\left({r\over L}\right)^2$$
15$$\xi={x\over L}\,\Rightarrow\quad for x\leq x\leq L then 0\leq\xi\leq 1$$
16$${d\over dx}\varphi(x) = \varphi^\prime(x) = {d\over d\xi}(\varphi(\xi)){d\xi\over x} = {1\over L}\varphi^\prime(\xi)$$
17$${d^2\over dx^2}\varphi(x) = \varphi^{(2)} = {1\over L^2}\varphi^{(2)}(\xi)$$
18$${d^3\over dx^3}\varphi(x) = \varphi^{(3)}(x) = {1\over L^3}\varphi^{(3)}(\xi)$$
19$${d^4\over dx^4}\varphi(x) = \varphi^{(4)}(x) = {1\over L^4}\varphi^{(4)}(\xi)$$
20$${EI\over L^4}\varphi^{(4)}(\xi) + {\omega^2\over L^2}\left(mr^2 + {mEI\over A_sG}\right)\varphi^{(2)}(\xi) + \left({m^2\omega^4r^2\over A_sG - m\omega^2}\right)\varphi(\xi) = 0$$
21$$\varphi^{(4)}(\xi) + b_n^2(R^2+a^2)\varphi^{(2)}(\xi) + b_n^2(a^2R^2b_n^2 - 1)\varphi(\xi) = 0$$
22$$\varphi^{(4)}(\xi) + b_n^2a^2\varphi^{(2)}(\xi) - b_n^2\varphi(\xi) = 0$$
23$$b_n^2(a^2R^2b_n^2-1)<0\Rightarrow(a^2R^2b_n^2 - 1)<0$$
24$$b_n^2(a^2R^2b_n^2 - 1) = 0\Rightarrow(a^2R^2b_n^2-1) = 0$$
25$$b_n^2(a^2R^2b_n^2 - 1)>0\Rightarrow(a^2R^2b_n^2-a)>0$$
26$$0<\omega<A\sqrt{kG\over mI}$$
27$$\omega = A\sqrt{kG\over mI}$$
28$$\omega>A\sqrt{kG\over mI}$$
29$$d^4+b_n^2(R^2+a^2)d^2+b_n^2(a^2R^2b_n^2-1) = 0$$
30$$d_{1,2} = \pm b$$
31$$d_{3,4} = \pm fi$$
32$$S_1=-1+\sqrt{1-{4(a^2R^2b_n^2-1)\over b_n^2(R^2+a^2)^2}}>0$$
33$$S_2=-1-\sqrt{1-{4(a^2R^2b_n^2-1)\over b_n^2(R^2+a^2)^2}}<0$$
34$$b=b_n\sqrt{{(R^2+a^2)\over 2}S_1}$$
35$$f=b_n\sqrt{-{(R^2+a^2)\over 2}S_2}$$
36$$\varphi(\xi) = A\sinh(b\xi) + B\cosh(b\xi) + C\sin(f\xi) + D\cos(f\xi)$$
37$$\varphi(\xi = 0) = 0$$
38$$\varphi^\prime(\xi = 0) = 0$$
39$$EI\varphi^{(2)}(\xi = 1) = 0$$
40$$EI\varphi^{(3)}(\xi = 1) - A_sG\varphi^\prime(\xi = 1) = 0$$
41$$(b^4 + f^4)EI + A_sG(f^2-b^2) + (bf(f^2-b^2)EI + 2bfA_sG)\sinh(b)\sin(f)+(2b^2f^2EI+A_sG(b^2-f^2))\cosh(b)\cos(f) = 0$$
42$$d^4+b_n^2(R^2 + a^2)d^2 = 0$$
43$$f=b_n\sqrt{(R^2 + a^2)}$$
44$$d_{1,2} = 0$$
45$$d_{3,4} = \pm fi$$
46$$\varphi(\xi) = A + B\xi + C\sin(f\xi) + D\cos(f\xi)$$
47$$f^2EI + A_sG(1 - \cos(f)) = 0$$
48$$d^2 = {b_n^2(R^2 + a^2)\over 2}\left(-1\pm\sqrt{1-{4(a^2R^2b_n^2 - 1)\over b_n^2(R^2+a^2)}}\right)$$
49$$(a^2R^2b_n^2-1)>0\Rightarrow 1-{4(a^2R^2b_n^2-1)\over b_n^2(R^2 + a^2)^2} < 1$$
50$$0<1-{4(a^2R^2b_n^2-1)\over b_n^2(R^2 + a^2)^2}<1$$
51$$1-{4(a^2R^2b_n^2-1)\over b_n^2(R^2 + a^2)^2} = 0$$
52$$1-{4(a^2R^2b_n^2-1)\over b_n^2(R^2 + a^2)^2} < 0$$
53$$b=b_n\sqrt{{(R^2+a^2)\over 2}\left(1-\sqrt{1-{4(a^2R^2b_n^2-1)\over b_n^2(R^2+a^2)^2}}\right)}$$
54$$f=b_n\sqrt{{(R^2+a^2)\over 2}\left(1+\sqrt{1-{4(a^2R^2b_n^2-1)\over b_n^2(R^2+a^2)^2}}\right)}$$
55$$d_{1,2} = \pm bi$$
56$$d_{3,4} = \pm fi$$
57$$\varphi(\xi) = A\sin(b\xi) + B\cos(b\xi) +C\sin(f\xi) + D\cos(f\xi)$$
58$$(b^4 + f^4)EI + A_sG(f^2+b^2) - bf(b^2EI+2A_sG+f^2EI)\sin(f)\sin(b)-(2b^2f^2EI + A_sG(b^2 + f^2))cos(b)cos(f) = 0$$
59$$b=b_n\sqrt{(R^2+a^2)\over 2}$$
60$$d_{1,2} = bi$$
61$$d_{3,4} = -bi$$
62$$\varphi(\xi) = A\sin(b\xi) + B\cos(b\xi) + C\xi\sin(b\xi) + D\xi\cos(b\xi)$$
63$$b^4EI + b^2A_sG+3b^2EI+b^2EI\cos^2(b)+A_sG\sin^2(b) = 0$$
64$$b=b_n\sqrt{(R^2+a^2)\over 2}\sqrt[4]{4(a^2R^2b_n^2 - 1)\over b_n^2(R^2+a^2)^2}\cos\left(\arctan(\beta)\over 2\right)$$
65$$f=b_n\sqrt{(R^2+a^2)\over 2}\sqrt[4]{4(a^2R^2b_n^2 - 1)\over b_n^2(R^2+a^2)^2}\sin\left(\arctan(\beta)\over 2\right)$$
66$$\beta = \sqrt{{4(a^2R^2b_n^2 - 1)\over b_n^2(R^2+a^2)^2} - 1}$$
67$$d_{1,2} = b\pm fi$$
68$$d_{3,4} = -b\pm fi$$
69$$\varphi(\xi) = e^{b\xi}(A\sin(f\xi) + B\cos(f\xi) + e^{-b\xi}(C\sin(f\xi) + D\cos(f\xi)))$$
70$$\begin{array}{l}
	(e^b)^2\left[-b^2f^2A_sG - f^6EI - f^4A_sG - 6b^4f^2EI\cos^2(f) - b^4f^2EI\right.\cr
	\ \left.+ 4f^4b^2EI\cos^2(f) - 2b^2f^4EI\sin^2(f) - 3b^5fEI\sin(f)\cos(f) + 6f^3b^3EI\sin(f)\cos(f)\right.\cr
	\ \left.- 3bf^5EI\sin(f)\cos(f)\right] + (e^{-b})^2\left[-b^4f^2EI-f^6EI-f^4A_sG-2f^4b^2EI\right.\cr
	\ \left.-b^2f^2A_sG\right] + (e^b)(e^{-b})\left[2f^4A_sG+2f^6EI+2b^2f^2A_sG\cos(2f)-6b^2f^4EI \right.\cr
	\ \left.-2b^2f^4EI\sin^2(f) - 6b^4f^2EI - 14b^4f^2EI\cos^2(f) + 4b^6EI\sin^2(f)\right.\cr
	\ \left.+ 3b^5fEI\sin(f)\cos(f) - 6b^3f^3EI\sin(f)\cos(f) + 3f^5bEI\sin(f)\cos(f)\right] = 0\cr\end{array}$$
71$$d^2 = {b_n^2a^2\over 2}\left(-1\pm\sqrt{1+{4\over b_n^2a^4}}\right)$$
72$$-1+\sqrt{1+{4\over b_n^2a^4}}>0$$
73$$-1-\sqrt{1+{4\over b_n^2a^4}}<0$$
74$$b={ab_n\over\sqrt{2}}\sqrt{-1+\sqrt{1+{4\over b_n^2a^4}}}$$
75$$f={ab_n\over\sqrt{2}}\sqrt{1+\sqrt{1+{4\over b_n^2a^4}}}$$
76$$d_{1,2} = \pm b$$
77$$d_{3,4} = \pm fi$$
78$$\varphi(\xi) = A\sinh(b\xi) + B\cosh(b\xi) +C\sin(f\xi) + D\cos(f\xi)$$
79$$\begin{array}{l}(b^4+f^4)EI + A_sG(f^2-b^2) + (bf(f^2-b^2)EI + 2bfA_sG)\sinh(b)\sinh(f)\cr
	\quad+(2b^2f^2EI+A_sG(b^2-f^2))\cosh(b)\cos(f) = 0\end{array}$$
80$${L\over r} = {L\over\sqrt{L_fL_w^3\over 12L_fL_w}} = {\sqrt{12}L\over L_w}$$
81$$W_b = \left[2A_b(L_f-H_b)+2A_b(L_w-H_b)\right]n\rho$$
82$$\begin{array}{l}W_c=\left[2A_c(y-H_b)\rho\left({L_f\over S} - 1\right)\right]n+\left[2A_c(y-H_b)\rho\left({L_w\over S} - 1\right)\right]n\cr
\qquad+\left[4LH_b^2\rho\right] + \left[4L(H_c - H_b)^2\rho\right]\end{array}$$
83$$W_s = \left[\left[L_f - H_b\right] - \left[4(H_c-H_b)^2\right]\right]t_s\rho n$$
84$$m = {W_b + W_c + W_s\over L}$$
85$$A = (L_fL_w) - (L_f-2t)(L_w-2t)$$
86$$A = 2t(L_f + L_w)$$
87$$I_z = {1\over 12}L_fL_w^3 - {1\over 12}(L_f - 2t)(L_w - 2t)^3$$
88$$I_z = {1\over 2}L_fL_w^2t+{1\over 6}L_w^3t$$
89$$k=-{2(1+v)\over\left[{A\over I_z^2}C_4 + v\left(1-{I_y\over I_z}\right)\right]}$$
90$$C_4 = -\int_A\left[v(f_1y^2 - f_1z^2 + 2f_2yz) + 2(1+v)(f_1^2+f_2^2)\right]dA$$
91$$\tau_{xy} = {V\over I_z}f_1(y,z)$$
92$$\tau_{xz} = {V\over I_z}f_2(y,z)$$
93$$k=-{2(1+v)\over \left[{9\over4a^5b}C_4 + v\left(1-{b^2\over a^2}\right)\right]}$$
94$$C_4 = {4\over 45}a^3b(-12a^2-15va^2+5vb^2) + \sum_{n=1}^{\infty}{16v^2b^5\left(n\pi a-b\tanh\left({n\pi a\over b}\right)\right)\over (n\pi)^5(1+v)}$$
